SStructTT/Dynamic/Substitution.lean
@@ -1,0 +1,85 @@
+import SStructTT.Static.Substitution
+import SStructTT.Dynamic.Renaming
+
+namespace Dynamic
+variable {Srt : Type} [inst : SStruct Srt]
+
+@[aesop safe (rule_sets := [subst]) [constructors]]
+inductive AgreeSubst : (Var -> Tm Srt) ->
+  Static.Ctx Srt -> Dynamic.Ctx Srt ->
+  Static.Ctx Srt -> Dynamic.Ctx Srt -> Prop
+where
+  | nil {σ} :
+    AgreeSubst σ [] [] [] []
+  | ex {Γ Γ' Δ Δ' A s i σ} :
+    Γ ⊢ A : .srt s i ->
+    AgreeSubst σ Γ Δ Γ' Δ' ->
+    AgreeSubst (up σ) (A :: Γ) (A :⟨s⟩ Δ) (A.[σ] :: Γ') (A.[σ] :⟨s⟩ Δ')
+  | im {Γ Γ' Δ Δ' A s i σ} :
+    Γ ⊢ A : .srt s i ->
+    AgreeSubst σ Γ Δ Γ' Δ' ->
+    AgreeSubst (up σ) (A :: Γ) (_: Δ) (A.[σ] :: Γ') (_: Δ')
+  | wk_im {Γ Γ' Δ Δ' A m σ} :
+    Γ' ⊢ m : A.[σ] ->
+    AgreeSubst σ Γ Δ Γ' Δ' ->
+    AgreeSubst (m .: σ) (A :: Γ) (_: Δ) Γ' Δ'
+  | wk_ex {Γ Γ' Δ Δ' Δa Δb A m s σ} :
+    Merge Δa Δb Δ' ->
+    Δa !≤ s ->
+    Γ' ;; Δa ⊢ m : A.[σ] ->
+    AgreeSubst σ Γ Δ Γ' Δb ->
+    AgreeSubst (m .: σ) (A :: Γ) (A :⟨s⟩ Δ) Γ' Δ'
+  | conv_im {Γ Γ' Δ Δ' A B s i σ} :
+    A === B ->
+    Γ ⊢ B : .srt s i ->
+    Γ' ⊢ B.[shift 1].[σ] : .srt s i ->
+    AgreeSubst σ (A :: Γ) (_: Δ) Γ' Δ' ->
+    AgreeSubst σ (B :: Γ) (_: Δ) Γ' Δ'
+  | conv_ex {Γ Γ' Δ Δ' A B s i σ} :
+    A === B ->
+    Γ ⊢ B : .srt s i ->
+    Γ' ⊢ B.[shift 1].[σ] : .srt s i ->
+    AgreeSubst σ (A :: Γ) (A :⟨s⟩ Δ) Γ' Δ' ->
+    AgreeSubst σ (B :: Γ) (B :⟨s⟩ Δ) Γ' Δ'
+
+lemma AgreeSubst.toStatic {Γ Γ'} {Δ Δ' : Ctx Srt} {σ} :
+    Dynamic.AgreeSubst σ Γ Δ Γ' Δ' -> Static.AgreeSubst σ Γ Γ' := by
+  intro agr
+  induction agr <;> try aesop (rule_sets := [subst])
+  case ex => constructor <;> assumption
+  case im => constructor <;> assumption
+  case wk_im => constructor <;> assumption
+  case wk_ex tym agr ih =>
+    constructor
+    . apply tym.toStatic
+    . assumption
+
+lemma AgreeSubst.none {Γ Γ'} {Δ Δ' : Ctx Srt} {σ} :
+    AgreeSubst σ Γ Δ Γ' Δ' -> Δ.Forall (. = none) -> Δ'.Forall (. = none) := by
+  intro agr h; induction agr
+  case nil => simp
+  case ex => simp at h
+  case im ih => simp at h; aesop
+  case wk_im ih => simp at h; aesop
+  case wk_ex => simp at h
+  case conv_im => simp at h; aesop
+  case conv_ex => simp at h
+
+lemma AgreeSubst.has {Γ Γ'} {Δ Δ' : Ctx Srt} {A x s σ} :
+    AgreeSubst σ Γ Δ Γ' Δ' -> Γ' ;; Δ' ⊢ -> Has Δ x s A -> Γ' ;; Δ' ⊢ (σ x) : A.[σ] := by
+  intro agr wf hs; induction agr generalizing x A
+  case nil => cases hs
+  case ex A s i σ tyA agr ih =>
+    cases hs
+    asimp
+    constructor
+    . assumption
+    . rw[show A.[σ !> shift 1] = A.[σ].[shift 1] by asimp]
+      constructor
+      sorry
+  case im A s i σ tyA agr ih =>
+    rcases wf with _ | _ | ⟨_, wf⟩
+    rcases hs with _ | @⟨_, A, s, x, hs⟩; asimp
+    rw[show A.[σ !> shift 1] = A.[σ].[shift 1] by asimp]
+    apply Typed.eweaken <;> try first | rfl | assumption
+    apply ih <;> assumption
